`StateGettersEquivalence.lean`: equivalence proofs for `gasPrice`

EvmEquivalence/Equivalence/StateGettersEquivalence.lean
@@ -16,6 +16,7 @@ inductive stateGetter_op where
   | address
   | origin
   | caller
+  | gasprice
 
 variable (op : stateGetter_op)
 
@@ -24,14 +25,18 @@ def stateGetter_op.to_binop : stateGetter_op → SortNullStackOp
   | .address  => .ADDRESS_EVM_NullStackOp
   | .origin => .ORIGIN_EVM_NullStackOp
   | .caller => .CALLER_EVM_NullStackOp
+  | .gasprice => .GASPRICE_EVM_NullStackOp
 
 def stateGetter_op.from_k : stateGetter_op → StateGettersSummary.stateGetter_op
  | .address  => .address
  | .origin => .origin
  | .caller => .caller
+ | .gasprice => .gasprice
 
 def oneOpLHS
   {GAS_CELL ID_CELL ORIGIN_CELL CALLER_CELL PC_CELL _Val6 _Val8 : SortInt}
+  -- We assume `GASPRICE_CELL` is not negative
+  {GASPRICE_CELL : ℕ}
   {SCHEDULE_CELL : SortSchedule}
   {USEGAS_CELL: SortBool}
   {WS : SortWordStack}
@@ -46,7 +51,6 @@ def oneOpLHS
   {_Gen14 : SortTouchedAccountsCell}
   {_Gen15 : SortVersionedHashesCell}
   {_Gen16 : SortSubstateCell}
-  {_Gen17 : SortGasPriceCell}
   {_Gen19 : SortBlockhashesCell}
   {_Gen20 : SortBlockCell}
   {_Gen21 : SortExitCodeCell}
@@ -89,7 +93,7 @@ def oneOpLHS
             callDepth := _Gen9 },
           versionedHashes := _Gen15,
           substate := _Gen16,
-          gasPrice := _Gen17,
+          gasPrice := { val := GASPRICE_CELL },
           origin := { val := (@inj SortInt SortAccount) ORIGIN_CELL },
           blockhashes := _Gen19,
           block := _Gen20 },
@@ -98,6 +102,8 @@ def oneOpLHS
 
 def oneOpRHS
   {TOP_STACK ID_CELL ORIGIN_CELL CALLER_CELL _Val6 _Val8 : SortInt}
+  -- We assume `GASPRICE_CELL` is not negative
+  {GASPRICE_CELL : ℕ}
   {SCHEDULE_CELL : SortSchedule}
   {WS : SortWordStack}
   {_DotVar0 : SortGeneratedCounterCell}
@@ -111,7 +117,6 @@ def oneOpRHS
   {_Gen14 : SortTouchedAccountsCell}
   {_Gen15 : SortVersionedHashesCell}
   {_Gen16 : SortSubstateCell}
-  {_Gen17 : SortGasPriceCell}
   {_Gen19 : SortBlockhashesCell}
   {_Gen20 : SortBlockCell}
   {_Gen21 : SortExitCodeCell}
@@ -154,7 +159,7 @@ def oneOpRHS
               callDepth := _Gen9 },
             versionedHashes := _Gen15,
             substate := _Gen16,
-            gasPrice := _Gen17,
+            gasPrice := { val := GASPRICE_CELL },
             origin := { val := (@inj SortInt SortAccount) ORIGIN_CELL },
             blockhashes := _Gen19,
             block := _Gen20 },
@@ -176,9 +181,12 @@ def stateGetter_op.do (tc : SortGeneratedTopCell) : SortInt :=
   | .address  => acc2Int tc.Iₐ.val
   | .origin => acc2Int tc.origin.val
   | .caller => acc2Int tc.caller.val
+  | .gasprice => Int.toNat tc.gasPrice.val
 
 theorem rw_oneOpLHS_oneOpRHS
   {GAS_CELL ID_CELL ORIGIN_CELL CALLER_CELL PC_CELL _Val0 _Val2 _Val6 _Val7 _Val8 : SortInt}
+  -- We assume `GASPRICE_CELL` is not negative
+  {GASPRICE_CELL : ℕ}
   {SCHEDULE_CELL : SortSchedule}
   {USEGAS_CELL _Val1 _Val3 _Val4 _Val5 : SortBool}
   {WS : SortWordStack}
@@ -216,10 +224,10 @@ theorem rw_oneOpLHS_oneOpRHS
   (defn_Val7 : «_<_>_SCHEDULE_Int_ScheduleConst_Schedule» SortScheduleConst.Gbase_SCHEDULE_ScheduleConst SCHEDULE_CELL = some _Val7)
   (defn_Val8 : «_-Int_» GAS_CELL _Val7 = some _Val8)
   (req : _Val5 = true):
-  let lhs := (@oneOpLHS op GAS_CELL ID_CELL ORIGIN_CELL CALLER_CELL PC_CELL _Val6 _Val8 SCHEDULE_CELL USEGAS_CELL WS _DotVar0 _DotVar2 _Gen0 _Gen1 _Gen10
-  _Gen11 _Gen12 _Gen13 _Gen14 _Gen15 _Gen16 _Gen17 _Gen19
+  let lhs := (@oneOpLHS op GAS_CELL ID_CELL ORIGIN_CELL CALLER_CELL PC_CELL _Val6 _Val8 GASPRICE_CELL SCHEDULE_CELL USEGAS_CELL WS _DotVar0 _DotVar2 _Gen0 _Gen1 _Gen10
+  _Gen11 _Gen12 _Gen13 _Gen14 _Gen15 _Gen16 _Gen19
   _Gen20 _Gen21 _Gen22 _Gen3 _Gen4 _Gen5 _Gen6 _Gen7 _Gen8 _Gen9 _K_CELL)
-  let rhs := (@oneOpRHS (op.do lhs) ID_CELL ORIGIN_CELL CALLER_CELL _Val6 _Val8 SCHEDULE_CELL WS _DotVar0 _DotVar2 _Gen0 _Gen1 _Gen10 _Gen11 _Gen12 _Gen13 _Gen14 _Gen15 _Gen16 _Gen17 _Gen19 _Gen20 _Gen21 _Gen22 _Gen3 _Gen4 _Gen5 _Gen6 _Gen7 _Gen8 _Gen9 _K_CELL)
+  let rhs := (@oneOpRHS (op.do lhs) ID_CELL ORIGIN_CELL CALLER_CELL _Val6 _Val8 GASPRICE_CELL SCHEDULE_CELL WS _DotVar0 _DotVar2 _Gen0 _Gen1 _Gen10 _Gen11 _Gen12 _Gen13 _Gen14 _Gen15 _Gen16 _Gen19 _Gen20 _Gen21 _Gen22 _Gen3 _Gen4 _Gen5 _Gen6 _Gen7 _Gen8 _Gen9 _K_CELL)
   Rewrites lhs rhs
    := by
   --intro lhs rhs; simp [lhs, rhs, oneOpLHS, oneOpRHS]
@@ -230,9 +238,13 @@ theorem rw_oneOpLHS_oneOpRHS
     <;> assumption
   . apply (@Rewrites.CALLER_SUMMARY_CALLER_SUMMARY_USEGAS CALLER_CELL GAS_CELL PC_CELL _Val0 _Val2)
     <;> assumption
+  . apply (@Rewrites.GASPRICE_SUMMARY_GASPRICE_SUMMARY_USEGAS GASPRICE_CELL GAS_CELL PC_CELL _Val0 _Val2)
+    <;> try assumption
 
 theorem oneOp_prestate_equiv
   {GAS_CELL ID_CELL ORIGIN_CELL CALLER_CELL PC_CELL _Val6 _Val8 : SortInt}
+  -- We assume `GASPRICE_CELL` is not negative
+  {GASPRICE_CELL : ℕ}
   {SCHEDULE_CELL : SortSchedule}
   {USEGAS_CELL: SortBool}
   {WS : SortWordStack}
@@ -247,7 +259,6 @@ theorem oneOp_prestate_equiv
   {_Gen14 : SortTouchedAccountsCell}
   {_Gen15 : SortVersionedHashesCell}
   {_Gen16 : SortSubstateCell}
-  {_Gen17 : SortGasPriceCell}
   {_Gen19 : SortBlockhashesCell}
   {_Gen20 : SortBlockCell}
   {_Gen21 : SortExitCodeCell}
@@ -261,8 +272,8 @@ theorem oneOp_prestate_equiv
   {_Gen9 : SortCallDepthCell}
   {_K_CELL : SortK}
   (symState : EVM.State):
-  let lhs := (@oneOpLHS op GAS_CELL ID_CELL ORIGIN_CELL CALLER_CELL PC_CELL _Val6 _Val8 SCHEDULE_CELL USEGAS_CELL WS _DotVar0 _DotVar2 _Gen0 _Gen1 _Gen10
-  _Gen11 _Gen12 _Gen13 _Gen14 _Gen15 _Gen16 _Gen17 _Gen19
+  let lhs := (@oneOpLHS op GAS_CELL ID_CELL ORIGIN_CELL CALLER_CELL PC_CELL _Val6 _Val8 GASPRICE_CELL SCHEDULE_CELL USEGAS_CELL WS _DotVar0 _DotVar2 _Gen0 _Gen1 _Gen10
+  _Gen11 _Gen12 _Gen13 _Gen14 _Gen15 _Gen16 _Gen19
   _Gen20 _Gen21 _Gen22 _Gen3 _Gen4 _Gen5 _Gen6 _Gen7 _Gen8 _Gen9 _K_CELL)
   stateMap symState lhs =
   {symState with
@@ -274,6 +285,7 @@ theorem oneOp_prestate_equiv
                   codeOwner := idMap lhs.Iₐ
                   sender := accountAddressMap lhs.origin.val
                   source := accountAddressMap lhs.caller.val
+                  gasPrice := GASPRICE_CELL
                   perm := !lhs.isStatic.val}
     accountMap := Axioms.SortAccountsCellMap lhs.accounts
     activeWords := intMap lhs.memoryUsed.val
@@ -289,6 +301,8 @@ theorem oneOp_prestate_equiv
 
 theorem oneOp_poststate_equiv
   {TOP_STACK ID_CELL ORIGIN_CELL CALLER_CELL PC_CELL _Val5 _Val6 _Val8 : SortInt}
+  -- We assume `GASPRICE_CELL` is not negative
+  {GASPRICE_CELL : ℕ}
   {SCHEDULE_CELL : SortSchedule}
   {WS : SortWordStack}
   {_DotVar0 : SortGeneratedCounterCell}
@@ -302,7 +316,6 @@ theorem oneOp_poststate_equiv
   {_Gen14 : SortTouchedAccountsCell}
   {_Gen15 : SortVersionedHashesCell}
   {_Gen16 : SortSubstateCell}
-  {_Gen17 : SortGasPriceCell}
   {_Gen19 : SortBlockhashesCell}
   {_Gen20 : SortBlockCell}
   {_Gen21 : SortExitCodeCell}
@@ -317,7 +330,7 @@ theorem oneOp_poststate_equiv
   {_K_CELL : SortK}
   (defn_Val6 : «_+Int_» PC_CELL 1 = some _Val6)
   (symState : EVM.State):
-  let rhs := (@oneOpRHS TOP_STACK ID_CELL ORIGIN_CELL CALLER_CELL _Val6 _Val8 SCHEDULE_CELL WS _DotVar0 _DotVar2 _Gen0 _Gen1 _Gen10 _Gen11 _Gen12 _Gen13 _Gen14 _Gen15 _Gen16 _Gen17 _Gen19 _Gen20 _Gen21 _Gen22 _Gen3 _Gen4 _Gen5 _Gen6 _Gen7 _Gen8 _Gen9 _K_CELL)
+  let rhs := (@oneOpRHS TOP_STACK ID_CELL ORIGIN_CELL CALLER_CELL _Val6 _Val8 GASPRICE_CELL SCHEDULE_CELL WS _DotVar0 _DotVar2 _Gen0 _Gen1 _Gen10 _Gen11 _Gen12 _Gen13 _Gen14 _Gen15 _Gen16 _Gen19 _Gen20 _Gen21 _Gen22 _Gen3 _Gen4 _Gen5 _Gen6 _Gen7 _Gen8 _Gen9 _K_CELL)
   stateMap symState rhs =
   {symState with
     stack := (intMap TOP_STACK) :: wordStackMap WS
@@ -328,6 +341,7 @@ theorem oneOp_poststate_equiv
                   codeOwner := idMap rhs.Iₐ,
                   sender := accountAddressMap rhs.origin.val
                   source := accountAddressMap rhs.caller.val
+                  gasPrice := GASPRICE_CELL
                   perm := !rhs.isStatic.val}
     accountMap := Axioms.SortAccountsCellMap rhs.accounts
     activeWords := intMap rhs.memoryUsed.val
@@ -351,6 +365,8 @@ attribute [local simp] GasConstants.Gbase
 -- This is because it doesn't include all semantics such as gas computation
 theorem step_oneOp_equiv
   {GAS_CELL ID_CELL ORIGIN_CELL CALLER_CELL PC_CELL _Val0 _Val2 _Val6 _Val7 _Val8 : SortInt}
+  -- We assume `GASPRICE_CELL` is not negative
+  {GASPRICE_CELL : ℕ}
   {SCHEDULE_CELL : SortSchedule}
   {USEGAS_CELL _Val1 _Val3 _Val4 _Val5 : SortBool}
   {WS : SortWordStack}
@@ -365,7 +381,6 @@ theorem step_oneOp_equiv
   {_Gen14 : SortTouchedAccountsCell}
   {_Gen15 : SortVersionedHashesCell}
   {_Gen16 : SortSubstateCell}
-  {_Gen17 : SortGasPriceCell}
   {_Gen19 : SortBlockhashesCell}
   {_Gen20 : SortBlockCell}
   {_Gen21 : SortExitCodeCell}
@@ -405,10 +420,10 @@ theorem step_oneOp_equiv
   (ORIGIN_CELL_nonneg : 0 ≤ ORIGIN_CELL)
   (CALLER_CELL_small : CALLER_CELL < AccountAddress.size)
   (CALLER_CELL_nonneg : 0 ≤ CALLER_CELL) :
-  let lhs := (@oneOpLHS op GAS_CELL ID_CELL ORIGIN_CELL CALLER_CELL PC_CELL _Val6 _Val8 SCHEDULE_CELL USEGAS_CELL WS _DotVar0 _DotVar2 _Gen0 _Gen1 _Gen10
-  _Gen11 _Gen12 _Gen13 _Gen14 _Gen15 _Gen16 _Gen17 _Gen19
+  let lhs := (@oneOpLHS op GAS_CELL ID_CELL ORIGIN_CELL CALLER_CELL PC_CELL _Val6 _Val8 GASPRICE_CELL SCHEDULE_CELL USEGAS_CELL WS _DotVar0 _DotVar2 _Gen0 _Gen1 _Gen10
+  _Gen11 _Gen12 _Gen13 _Gen14 _Gen15 _Gen16 _Gen19
   _Gen20 _Gen21 _Gen22 _Gen3 _Gen4 _Gen5 _Gen6 _Gen7 _Gen8 _Gen9 _K_CELL)
-  let rhs := (@oneOpRHS (op.do lhs) ID_CELL ORIGIN_CELL CALLER_CELL _Val6 _Val8 SCHEDULE_CELL WS _DotVar0 _DotVar2 _Gen0 _Gen1 _Gen10 _Gen11 _Gen12 _Gen13 _Gen14 _Gen15 _Gen16 _Gen17 _Gen19 _Gen20 _Gen21 _Gen22 _Gen3 _Gen4 _Gen5 _Gen6 _Gen7 _Gen8 _Gen9 _K_CELL)
+  let rhs := (@oneOpRHS (op.do lhs) ID_CELL ORIGIN_CELL CALLER_CELL _Val6 _Val8 GASPRICE_CELL SCHEDULE_CELL WS _DotVar0 _DotVar2 _Gen0 _Gen1 _Gen10 _Gen11 _Gen12 _Gen13 _Gen14 _Gen15 _Gen16  _Gen19 _Gen20 _Gen21 _Gen22 _Gen3 _Gen4 _Gen5 _Gen6 _Gen7 _Gen8 _Gen9 _K_CELL)
   EVM.step_arith op.from_k gas gasCost (stateMap symState lhs) =
   .ok (stateMap {symState with execLength := symState.execLength + 1} rhs) := by
   intro lhs rhs
@@ -448,6 +463,8 @@ attribute [local simp] GasConstants.Glow
  -/
 theorem X_oneOp_equiv
   {GAS_CELL ID_CELL ORIGIN_CELL CALLER_CELL PC_CELL _Val0 _Val2 _Val6 _Val7 _Val8 : SortInt}
+  -- We assume `GASPRICE_CELL` is not negative
+  {GASPRICE_CELL : ℕ}
   {SCHEDULE_CELL : SortSchedule}
   {USEGAS_CELL _Val1 _Val3 _Val4 _Val5 : SortBool}
   {WS : SortWordStack}
@@ -462,7 +479,6 @@ theorem X_oneOp_equiv
   {_Gen14 : SortTouchedAccountsCell}
   {_Gen15 : SortVersionedHashesCell}
   {_Gen16 : SortSubstateCell}
-  {_Gen17 : SortGasPriceCell}
   {_Gen19 : SortBlockhashesCell}
   {_Gen2 : SortCallerCell}
   {_Gen20 : SortBlockCell}
@@ -502,10 +518,10 @@ theorem X_oneOp_equiv
   (ORIGIN_CELL_nonneg : 0 ≤ ORIGIN_CELL)
   (CALLER_CELL_small : CALLER_CELL < AccountAddress.size)
   (CALLER_CELL_nonneg : 0 ≤ CALLER_CELL) :
-  let lhs := (@oneOpLHS op GAS_CELL ID_CELL ORIGIN_CELL CALLER_CELL PC_CELL _Val6 _Val8 SCHEDULE_CELL USEGAS_CELL WS _DotVar0 _DotVar2 _Gen0 _Gen1 _Gen10
-  _Gen11 _Gen12 _Gen13 _Gen14 _Gen15 _Gen16 _Gen17 _Gen19
+  let lhs := (@oneOpLHS op GAS_CELL ID_CELL ORIGIN_CELL CALLER_CELL PC_CELL _Val6 _Val8 GASPRICE_CELL SCHEDULE_CELL USEGAS_CELL WS _DotVar0 _DotVar2 _Gen0 _Gen1 _Gen10
+  _Gen11 _Gen12 _Gen13 _Gen14 _Gen15 _Gen16 _Gen19
   _Gen20 _Gen21 _Gen22 _Gen3 _Gen4 _Gen5 _Gen6 _Gen7 _Gen8 _Gen9 _K_CELL)
-  let rhs := (@oneOpRHS (op.do lhs) ID_CELL ORIGIN_CELL CALLER_CELL _Val6 _Val8 SCHEDULE_CELL WS _DotVar0 _DotVar2 _Gen0 _Gen1 ⟨.empty⟩ _Gen11 _Gen12 _Gen13 _Gen14 _Gen15 _Gen16 _Gen17 _Gen19 _Gen20 _Gen21 _Gen22 _Gen3 _Gen4 _Gen5 _Gen6 _Gen7 _Gen8 _Gen9 _K_CELL)
+  let rhs := (@oneOpRHS (op.do lhs) ID_CELL ORIGIN_CELL CALLER_CELL _Val6 _Val8 GASPRICE_CELL SCHEDULE_CELL WS _DotVar0 _DotVar2 _Gen0 _Gen1 ⟨.empty⟩ _Gen11 _Gen12 _Gen13 _Gen14 _Gen15 _Gen16 _Gen19 _Gen20 _Gen21 _Gen22 _Gen3 _Gen4 _Gen5 _Gen6 _Gen7 _Gen8 _Gen9 _K_CELL)
   EVM.X (UInt256.toNat (intMap GAS_CELL)) symValidJumps
   (stateMap symState lhs) =
   .ok (.success (stateMap {symState with execLength := symState.execLength + 2} rhs) ByteArray.empty) := by
